src/tls/DefineTable.fst
@@ -96,8 +96,6 @@ let lemma_forall_empty #it #vt t pred h = ()
 
 let lemma_forall_elim #it #vt t pred h #i k = ()
 
-let lemma_forall_restore #it #vt t pred fp #i k h0 h1 = admit ()
-
 let lemma_forall_extend #it #vt t pred fp pred_frame #i k h0 h1 =
   if model then
     let prove_on_witness (x:it) (y:vt x{defined_as t y h1})
@@ -110,6 +108,8 @@ let lemma_forall_extend #it #vt t pred fp pred_frame #i k h0 h1 =
       ) in
     FStar.Classical.forall_intro_2 prove_on_witness
   else ()
+
+let lemma_forall_restore #it #vt t pred fp pred_frame #i k h0 h1 = admit ()
 
 let lemma_forall_frame #it #vt t pred fp pred_frame h0 l h1 =
   if model then 
