src/tls/ParsersAux.Binders.Aux.fst
@@ -71,9 +71,9 @@ let serialize_clientHello_eq
 = LP.serialize_synth_eq _ CH.synth_clientHello CH.clientHello'_serializer CH.synth_clientHello_recip () c;
   LP.serialize_nondep_then_eq
     ((Parsers.ProtocolVersion.protocolVersion_serializer `LP.serialize_nondep_then` Parsers.Random.random_serializer) `LP.serialize_nondep_then` (Parsers.SessionID.sessionID_serializer `LP.serialize_nondep_then` CH.clientHello_cipher_suites_serializer))
-    (CH.clientHello_compression_method_serializer `LP.serialize_nondep_then` CHEs.clientHelloExtensions_serializer)
+    (CH.clientHello_compression_methods_serializer `LP.serialize_nondep_then` CHEs.clientHelloExtensions_serializer)
     (((c.CH.version, c.CH.random), (c.CH.session_id, c.CH.cipher_suites)),
-    (c.CH.compression_method, c.CH.extensions));
+    (c.CH.compression_methods, c.CH.extensions));
   LP.serialize_nondep_then_eq
     (Parsers.ProtocolVersion.protocolVersion_serializer `LP.serialize_nondep_then` Parsers.Random.random_serializer)
     (Parsers.SessionID.sessionID_serializer `LP.serialize_nondep_then` CH.clientHello_cipher_suites_serializer)
@@ -87,9 +87,9 @@ let serialize_clientHello_eq
     CH.clientHello_cipher_suites_serializer
     (c.CH.session_id, c.CH.cipher_suites);
   LP.serialize_nondep_then_eq
-    CH.clientHello_compression_method_serializer
+    CH.clientHello_compression_methods_serializer
     CHEs.clientHelloExtensions_serializer
-    (c.CH.compression_method, c.CH.extensions)
+    (c.CH.compression_methods, c.CH.extensions)
 
 let serialize_handshake_m_client_hello_eq
   c
